\begin{enumerate}[label=\thesection.\arabic*.,ref=\thesection.\theenumi]
\numberwithin{equation}{enumi}
\item
\begin{align}
 \dot{x(t)}=\bm{A}x(t)+\bm{B}u(t) \\
 y(t)=\bm{C}x(t)+Du(t)
\end{align} 
Taking Laplace transform on both sides we have the following equations
\begin{align}
s\bm{I}X(s)-x(0)= \bm{A}X(s)+ \bm{B}U(s)\\
(s\bm{I}-\bm{A})X(s)= \bm{B}U(s)+ x(0)\\
X(s)={(s\bm{I}-\bm{A})^{-1}}\bm{B} U(s)+ (s\bm{I}-\bm{A})^{-1}x(0)
\end{align}
and
\begin{align}
Y(s)= \bm{C}X(s)+D\bm{I}U(s)
\end{align}
substituting 0.1.1 in this equation gives
\begin{align}
Y(s)=( \bm{C}{(s\bm{I}-\bm{A})^{-1}}\bm{B}+D\bm{I}) U(s) + \bm{C}(s\bm{I}-\bm{A})^{-1}x(0)
\end{align}
Assuming initially system was at rest i.e x(0)=0
\begin{align}
H(s)= {\frac{Y(s)}{U(s)}}= \bm{C}{(s\bm{I}-\bm{A})^{-1}}\bm{B}+D\bm{I}
\end{align}
Given,D=0 and \bm{B}= {\myvec{0\\0\\1}}

\begin{align}
H(s)=\frac{1}{s^3 + 3s^2+2s + 1}
\end{align}

Now, 
\begin{align} 
{\frac{Y(s)}{U(s)}}= {\frac{\frac{Y(s)}{X(s)}}{\frac{U(s)}{X(s)}}}  
\end{align}
We get
\begin{align}
 {\frac{Y(s)}{X(s)}}= 1
\end{align}
and
\begin{align}
{\frac{U(s)}{X(s)}}={s^3 + 3s^2+2s + 1}
\end{align}

giving
\begin{align}
U(s)= s^3 X(s) + 3s^2 X(s)+2sX(s) + X(s)
\end{align}

so equation 0.1.13 can be written as
\begin{align}
\myvec{sX(s)\\s^2X(s)\\s^3X(s)}
=
\myvec{0&1&0\\0&0&1\\-1&-2&-3}\myvec{X(s)\\s(s)\\s^2X(s)}
+
\myvec{0\\0\\1}  U
\end{align}
So \bm{A}=\myvec{0&1&0\\0&0&1\\-1&-2&-3}

\begin{align}
Y=X_{1}(s)
=\myvec{1&0&0} \myvec{X(s)\\sX(s)\\s^2X(s)}
\end{align}
\begin{align}
\bm{C}=\myvec{1&0&0}
\end{align}
\end{enumerate}